compiler/util/date_time_component.mli
@@ -1,0 +1,129 @@
+(*
+ * Licensed under the Apache License, Version 2.0 (the "License");
+ * you may not use this file except in compliance with the License.
+ * You may obtain a copy of the License at
+ *
+ * http://www.apache.org/licenses/LICENSE-2.0
+ *
+ * Unless required by applicable law or agreed to in writing, software
+ * distributed under the License is distributed on an "AS IS" BASIS,
+ * WITHOUT WARRANTIES OR CONDITIONS OF ANY KIND, either express or implied.
+ * See the License for the specific language governing permissions and
+ * limitations under the License.
+ *)
+
+(** Native OCaml support for the Ergo DateTime library *)
+
+(** Formats *)
+(** Those are taken from the Accord Project specification:
+YYYY         2014               4 or 2 digit year
+YY           14                 2 digit year
+MMMM         December           Long month name
+MMM          Feb.               Short month name
+MM           04                 2 digit month number
+M            12                 1 or 2 digit month number
+DD           04                 2 digit day of month
+D            3                  1 or 2 digit day of month
+HH           04                 2 digit hours
+H            3                  1 or 2 digit hours
+mm           59                 2 digit minutes
+ss           34                 2 digit seconds
+SSS          002                3 digit milliseconds
+Z            +01:00             UTC offset
+*)
+
+type date_time_format
+val format_eq : date_time_format -> date_time_format -> bool
+val format_from_string : string -> date_time_format
+
+(** Duration *)
+type duration
+val duration_eq : duration -> duration -> bool
+val duration_to_string : duration -> string
+val duration_from_string : string -> duration
+val duration_amount : duration -> int
+
+val duration_from_seconds : int -> duration
+val duration_from_minutes : int -> duration
+val duration_from_hours : int -> duration
+val duration_from_days : int -> duration
+val duration_from_weeks : int -> duration
+
+val duration_seconds : int -> duration
+val duration_minutes : int -> duration
+val duration_hours : int -> duration
+val duration_days : int -> duration
+val duration_weeks : int -> duration
+
+(** Period *)
+type period
+val period_eq : period -> period -> bool
+val period_to_string : period -> string
+val period_from_string : string -> period
+
+val period_from_days : int -> period
+val period_from_weeks : int -> period
+val period_from_months : int -> period
+val period_from_quarters : int -> period
+val period_from_years : int -> period
+
+val period_days : int -> period
+val period_weeks : int -> period
+val period_months : int -> period
+val period_quarters : int -> period
+val period_years : int -> period
+
+(** DateTime *)
+type dateTime
+val eq : dateTime -> dateTime -> bool
+
+(** Initial *)
+val now : unit -> dateTime
+
+(** Serialize/deserialize *)
+val from_string : string -> dateTime
+val format_to_string : date_time_format -> string
+val to_string_format : dateTime -> date_time_format -> string
+
+(** Components *)
+val get_seconds : dateTime -> int
+val get_minutes : dateTime -> int
+val get_hours : dateTime -> int
+val get_days : dateTime -> int
+val get_weeks : dateTime -> int
+val get_months : dateTime -> int
+val get_quarters : dateTime -> int
+val get_years : dateTime -> int
+
+(** Min/Max *)
+val max : dateTime list -> dateTime
+val min : dateTime list -> dateTime
+
+(** Comparisons *)
+val is_before : dateTime -> dateTime -> bool
+val is_after : dateTime -> dateTime -> bool
+
+(** Start/End of period *)
+val start_of_day : dateTime -> dateTime
+val start_of_week : dateTime -> dateTime
+val start_of_month : dateTime -> dateTime
+val start_of_quarter : dateTime -> dateTime
+val start_of_year : dateTime -> dateTime
+
+val end_of_day : dateTime -> dateTime
+val end_of_week : dateTime -> dateTime
+val end_of_month : dateTime -> dateTime
+val end_of_quarter : dateTime -> dateTime
+val end_of_year : dateTime -> dateTime
+
+(** Arithmetics *)
+val diff : dateTime -> dateTime -> duration
+val diff_days : dateTime -> dateTime -> float
+val diff_seconds : dateTime -> dateTime -> float
+
+val add : dateTime -> duration -> dateTime
+val subtract : dateTime -> duration -> dateTime
+
+val add_period : dateTime -> period -> dateTime
+val subtract_period : dateTime -> period -> dateTime
+
