compiler/core/ErgoWasm/Lang/ErgoWasm.v
@@ -1,0 +1,42 @@
+(*
+ * Licensed under the Apache License, Version 2.0 (the "License");
+ * you may not use this file except in compliance with the License.
+ * You may obtain a copy of the License at
+ *
+ * http://www.apache.org/licenses/LICENSE-2.0
+ *
+ * Unless required by applicable law or agreed to in writing, software
+ * distributed under the License is distributed on an "AS IS" BASIS,
+ * WITHOUT WARRANTIES OR CONDITIONS OF ANY KIND, either express or implied.
+ * See the License for the specific language governing permissions and
+ * limitations under the License.
+ *)
+
+(** ErgoWasm is an IL for Wasm *)
+
+(** * Abstract Syntax *)
+
+Require Import String.
+Require Import List.
+Require Import Qcert.Driver.CompEval.
+Require Import Qcert.EJson.Model.ForeignEJson.
+Require Import Qcert.EJson.Model.EJson.
+Require Import Qcert.WasmAst.Lang.WasmAst.
+Require Import ErgoSpec.Backend.QLib.
+Require Import ErgoSpec.Common.Provenance.
+Require Import ErgoSpec.Common.Result.
+
+Section ErgoWasm.
+  Context {m : brand_model}.
+
+  (** WASM programs are in AST form *)
+  (** Same type as in Q*cert *)
+  Definition wasm_ast := wasm_ast.
+  Definition wasm_ast_eval := wasm_ast_eval.
+  Axiom wasm_ast_to_string : wasm_ast -> nstring.
+
+End ErgoWasm.
+
+Extract Constant wasm_ast => "Qcert_lib.Wasm_ast.t".
+Extract Constant wasm_ast_eval => "Qcert_lib.Wasm_ast.eval".
+Extract Constant wasm_ast_to_string => "Qcert_lib.Wasm_ast.to_string".
