compiler/core/Translation/ErgoImptoWasm.v
@@ -1,0 +1,44 @@
+(*
+ * Licensed under the Apache License, Version 2.0 (the "License");
+ * you may not use this file except in compliance with the License.
+ * You may obtain a copy of the License at
+ *
+ * http://www.apache.org/licenses/LICENSE-2.0
+ *
+ * Unless required by applicable law or agreed to in writing, software
+ * distributed under the License is distributed on an "AS IS" BASIS,
+ * WITHOUT WARRANTIES OR CONDITIONS OF ANY KIND, either express or implied.
+ * See the License for the specific language governing permissions and
+ * limitations under the License.
+ *)
+
+(** Translates ErgoNNRC to JavaScript *)
+
+Require Import String.
+Require Import List.
+
+Require Import Qcert.JavaScriptAst.JavaScriptAstRuntime.
+Require Import Qcert.Driver.CompDriver.
+Require Import ErgoSpec.Version.
+Require Import ErgoSpec.Utils.Misc.
+Require Import ErgoSpec.Common.Result.
+Require Import ErgoSpec.Common.Names.
+Require Import ErgoSpec.Types.ErgoType.
+Require Import ErgoSpec.ErgoImp.Lang.ErgoImp.
+Require Import ErgoSpec.Backend.QLib.
+Require Import ErgoSpec.ErgoWasm.Lang.ErgoWasm.
+
+Section ErgoImptoWasm.
+  Local Open Scope list_scope.
+
+  Context {bm:brand_model}.
+
+  Axiom ergo_imp_ejson_to_wasm_ast : ergo_imp_module -> wasm_ast.
+
+  Definition ergo_imp_module_to_wasm
+             (contract_name:string)
+             (p:ergo_imp_module) : wasm_ast :=
+    ergo_imp_ejson_to_wasm_ast p.
+End ErgoImptoWasm.
+
+Extract Constant ergo_imp_ejson_to_wasm_ast => "Ergo_wasm_translate.ergo_imp".
